Prop monad version of typing

src/Typing.v
@@ -4,11 +4,16 @@ From Heapster Require Import
      PropT.
 
 From Coq Require Import
+     Ensembles
      Classes.Morphisms
      Classes.RelationClasses
      Relations.Relation_Operators
      Relations.Operators_Properties
      Program.Equality.
+
+From ExtLib Require Import
+     Structures.Functor
+     Structures.Monad.
 
 From ITree Require Import
      ITree
@@ -25,11 +30,91 @@ From Paco Require Import
 Import ITreeNotations.
 Import ITree.Basics.Basics.Monads.
 
+Global Instance EqM_Prop : EqM Ensembles.Ensemble := Ensembles.Same_set.
+
+Global Instance Functor_Prop : Functor.Functor Ensembles.Ensemble :=
+  {| fmap := fun _ _ f Pa b => exists a, Pa a /\ f a = b |}.
+
+Global Instance Monad_Prop : Monad Ensembles.Ensemble :=
+  {|
+  ret := fun _ x y => x = y;
+  bind := fun _ _ Pa K b => exists a, In _ Pa a /\ In _ (K a) b
+  |}.
+
+Lemma bind_ret_l_Prop : forall A B (f : A -> Ensembles.Ensemble B) a,
+    eqm (bind (ret a) f) (f a).
+Proof.
+  split; repeat intro; simpl in *.
+  - destruct H as (? & ? & ?). red in H. subst; auto.
+  - eexists; split; eauto. reflexivity.
+Qed.
+
+Lemma bind_ret_r_Prop : forall (A : Type) (Pa : Ensembles.Ensemble A),
+    eqm (bind Pa (fun a => ret a)) Pa.
+Proof.
+  split. repeat intro; simpl in *.
+  - destruct H as (? & ? & ?). red in H0; subst; auto.
+  - red. repeat intro. eexists; split; eauto. reflexivity.
+Qed.
+
+Lemma bind_bind_Prop :
+  forall A B C (Pa : Ensembles.Ensemble A)
+    (f : A -> Ensembles.Ensemble B) (g : B -> Ensembles.Ensemble C),
+    eqm (bind (bind Pa f) g) (bind Pa (fun y => bind (f y) g)).
+Proof.
+  intros. split; repeat intro; simpl in *;
+            [destruct H as (? & (? & ? & ?) & ?) | destruct H as (? & ? & (? & ? & ?))];
+            do 2 (eexists; split; eauto).
+Qed.
+
+Definition PropM (T : Type) (R : Type) := Ensembles.Ensemble (T * R).
+Global Instance EqM_PropM T : EqM (PropM T) := fun _ => Ensembles.Same_set _.
+
+Global Instance Functor_PropM T : Functor.Functor (PropM T) :=
+  {|
+  fmap := fun A B (f : A -> B) (Pa : PropM T A) (pb : T * B) =>
+            exists (pa : T * A), Pa pa /\ (fst pa, f (snd pa)) = pb
+  |}.
+
+Global Instance Monad_PropM T : Monad (PropM T) :=
+  {|
+  ret := fun A a pa => a = snd pa;
+  bind := fun A B (Pa : PropM T A) (K : A -> PropM T B) (pb : T * B) =>
+            exists (a : A), In _ Pa (fst pb, a) /\ In _ (K a) pb
+  |}.
+
+Lemma bind_ret_l_PropM : forall T A B (f : A -> PropM T B) a,
+    eqm (bind (ret a) f) (f a).
+Proof.
+  split; repeat intro; simpl in *.
+  - destruct H as (? & ? & ?). red in H. subst. auto.
+  - exists a; split; [split |]; auto.
+Qed.
+
+Lemma bind_ret_r_PropM : forall T (A : Type) (Pa : PropM T A),
+    eqm (bind Pa (fun a => ret a)) Pa.
+Proof.
+  split; repeat intro; simpl in *.
+  - destruct H as (? & ? & ?). red in H0. destruct x; subst; auto.
+  - exists (snd x); split; auto; destruct x; red; auto.
+Qed.
+
+Lemma bind_bind_PropM :
+  forall T A B C (Pa : PropM T A)
+    (f : A -> PropM T B) (g : B -> PropM T C),
+    eqm (bind (bind Pa f) g) (bind Pa (fun y => bind (f y) g)).
+Proof.
+  intros. split; repeat intro; simpl in *;
+            [destruct H as (? & (? & ? & ?) & ?) | destruct H as (? & ? & (? & ? & ?))];
+            do 2 (eexists; split; eauto).
+Qed.
+
 Section ts.
 
   Definition E := (stateE config +' nondetE).
 
-  Context {R : Type}.
+  (* Context {R : Type}. *)
+  Definition R := nat.
 
   Definition par_match
              (par : itree E R -> itree E R -> itree E R)
@@ -56,6 +141,13 @@ Section ts.
     intros. apply bisimulation_is_eq. revert t1 t2.
     ginit. gcofix CIH. intros. gstep. unfold par. constructor. red. intros.
     apply Reflexive_eqit_gen_eq. (* not sure why reflexivity doesn't work here *)
+  Qed.
+
+  Lemma rewrite_spin : (ITree.spin : itree E R) = Tau (ITree.spin).
+  Proof.
+    intros. apply bisimulation_is_eq.
+    ginit. gcofix CIH. gstep. unfold ITree.spin. constructor.
+    apply Reflexive_eqit_gen_eq.
   Qed.
 
   Variant step : itree E R -> config -> itree E R -> config -> Prop :=
@@ -156,6 +248,113 @@ Section ts.
     - symmetry. auto.
   Qed.
 
+  CoInductive iter_PropM_perm {R I : Type} (step : I -> PropM perm (I + R)) (i : I) (pr : perm * R)
+    : Prop :=
+  | iter_done
+    : step i (fst pr, (inr (snd pr))) -> iter_PropM_perm step i pr
+  | iter_step i'
+    : let p := fst pr in
+      let r := snd pr in
+      step i (p, (inl i')) ->
+      (exists p', sep_step p p' /\
+             iter_PropM_perm step i' (p', r)) ->
+      iter_PropM_perm step i pr
+  .
+  Global Instance MonadIter_PropM : MonadIter (PropM perm) := @iter_PropM_perm.
+
+  Definition h_nondet : nondetE ~> stateT config (PropM perm) :=
+    fun R e c =>
+      fun (pcr : perm * (config * R)) =>
+        let p := fst pcr in
+        let c' := fst (snd pcr) in
+        let r := snd (snd pcr) in
+        dom p c ->
+        c = c' /\
+        match e in (nondetE bool) return bool -> Prop with
+        | Or => fun r => r = true \/ r = false
+        end r.
+
+  Definition h_state : stateE config ~> stateT config (PropM perm) :=
+    fun R e c =>
+      fun (pcr : perm * (config * R)) =>
+        let p := fst pcr in
+        let c' := fst (snd pcr) in
+        let r := snd (snd pcr) in
+        dom p c ->
+        match e in (stateE _ X) return X -> Prop with
+        | Get _ => fun r => c' = c /\ r = c
+        | Put _ c'' => fun r =>
+                        upd p c c' /\ (* true for all other cases since c = c' there *)
+                        c' = c'' /\
+                        r = tt
+        end r.
+
+
+  Lemma h_nondet_lte R e c p q r :
+    p <= q -> h_nondet R e c (p, r) -> h_nondet R e c (q, r).
+  Proof.
+    intros. destruct e; repeat intro; simpl in *.
+    apply H0; auto. apply H; auto.
+  Qed.
+  Lemma h_state_lte R e c p q r :
+    p <= q -> h_state R e c (p, r) -> h_state R e c (q, r).
+  Proof.
+    intros. destruct e; repeat intro; simpl in *.
+    - apply H0; auto. apply H; auto.
+    - destruct H0 as (? & ? & ?).
+      + apply H; auto.
+      + split; auto. apply H; auto.
+  Qed.
+
+  Definition handler : E ~> stateT config (PropM perm) := case_ h_state h_nondet.
+
+  Definition test1 := par (Ret 0) (Ret 1).
+  Definition test2 : itree E R := Ret 1.
+  Definition test_interp := interp handler test2.
+
+  Definition empty_config := Build_config nil.
+  Eval cbv in test_interp empty_config.
+
+  Goal forall p c (n : R), interp handler (Ret n) c (p, (c, n)).
+  Proof.
+    intros. repeat red. constructor. repeat red. cbn. eexists. split; auto.
+  Qed.
+
+  Goal forall p q (t : itree E R) c n,
+      interp handler t c (p, (c, n)) -> p <= q -> interp handler t c (q, (c, n)).
+  Proof.
+    intros. repeat red in H. destruct H; auto.
+    - constructor 1. simpl in *. decompose [ex and] H; clear H.
+      exists x; split; auto. destruct x. repeat red. repeat red in H3; simpl in *.
+      destruct s; inversion H3. subst.
+      unfold observe in H2. destruct (_observe t0); simpl; auto.
+      red in H2. decompose [ex and] H2; clear H2. inversion H4.
+    - simpl in p0, r. replace p0 with p in H, H1; auto. clear p0.
+      replace r with (c, n) in H1; auto. clear r.
+      econstructor 2.
+      + repeat red. clear H1. repeat red in H. decompose [ex and] H; clear H.
+        exists x. destruct x. split; auto.
+        * clear H3. simpl in *. destruct (observe t0); simpl in *; auto. repeat red in H2 |- *.
+          decompose [ex and] H2; clear H2. destruct x as (? & ? & ?).
+          inversion H3; clear H3; subst.
+          exists (q, (c0, x)). split; auto.
+          destruct e; [eapply h_state_lte | eapply h_nondet_lte]; eauto.
+        * clear H2. repeat red in H3 |- *; simpl in *. destruct s; inversion H3.
+          f_equal.
+      + decompose [ex and] H1; clear H1. exists x. split; auto. eapply sep_step_lte; eauto.
+  Qed.
+
+  Goal forall p c n,
+      interp handler (ITree.spin : itree E R) c (p, (c, n)).
+  Proof.
+    repeat red. cofix CIH.
+    econstructor 2.
+    - repeat red. eexists; split; repeat red; simpl.
+      + rewrite rewrite_spin. simpl. auto.
+      + simpl. auto.
+    - exists p. split; simpl; intuition.
+  Qed.
+
   Variant typing_perm_gen typing (p : perm) (t : itree E R) : Prop :=
   | cond : (forall c, dom p c ->
                  forall t' c',
@@ -177,13 +376,6 @@ Section ts.
   Qed.
   Hint Resolve typing_perm_gen_mon : paco.
 
-  Lemma rewrite_spin : (ITree.spin : itree E R) = Tau (ITree.spin).
-  Proof.
-    intros. apply bisimulation_is_eq.
-    ginit. gcofix CIH. gstep. unfold ITree.spin. constructor.
-    apply Reflexive_eqit_gen_eq.
-  Qed.
-
   Lemma typing_perm_lte : forall p q t, typing_perm p t -> p <= q -> typing_perm q t.
   Proof.
     intros. pcofix CIH. pstep. constructor; intros.
@@ -191,6 +383,13 @@ Section ts.
     destruct H5 as [p' [? [? ?]]]. exists p'. split; [| split]; auto.
     - pclearbot. left. eapply paco2_mon_bot; eauto.
     - eapply sep_step_lte; eauto.
+  Qed.
+
+  Lemma typing_perm_spin : forall p, typing_perm p ITree.spin.
+  Proof.
+    pcofix CIH. pstep. constructor. intros. rewrite rewrite_spin in H0.
+    inversion H0; subst; split; try reflexivity.
+    exists p. split; eauto; intuition.
   Qed.
 
   Definition typing P t := forall p, p ∈ P -> typing_perm p t.
@@ -202,9 +401,7 @@ Section ts.
 
   Lemma type_spin : forall P, typing P ITree.spin.
   Proof.
-    pcofix CIH. intros. pstep. constructor. intros. rewrite rewrite_spin in H1.
-    inversion H1; subst. split; try reflexivity.
-    exists p. split; eauto; intuition.
+    repeat intro. apply typing_perm_spin.
   Qed.
 
   Lemma type_ret : forall P r, typing P (Ret r).
